theories/Terms.v
@@ -1,7 +1,12 @@
 From Coq Require Import
-  String.
+  String
+  List
+  Classes.EquivDec.
 From LambdaST Require Import
   Ident.
+
+
+From LambdaST Require Import Types.
 
 Declare Scope term_scope.
 
@@ -13,7 +18,7 @@ Inductive term : Set :=
   | TmSemic (lhs rhs : term)
   | TmLet (bind : ident) (bound body : term)
   | TmLetPar (lhs rhs bound : ident) (body : term) 
-  | TmLetCat (lhs rhs bound : ident) (body : term) 
+  | TmLetCat (t : type) (lhs rhs bound : ident) (body : term) 
   .
 
 Bind Scope term_scope with term.
@@ -27,8 +32,42 @@ Notation "'let' x = bound 'in' body" :=
   (TmLet x bound body) (at level 98, right associativity) : term_scope.
 Notation "'let' ( lhs , rhs ) = both 'in' body" :=
   (TmLetPar lhs rhs both body) (at level 98, right associativity) : term_scope.
-Notation "'let' ( lhs ; rhs ) = both 'in' body" :=
-  (TmLetCat lhs rhs both body) (at level 98, right associativity) : term_scope.
+Notation "'let' t ( lhs ; rhs ) = both 'in' body" :=
+  (TmLetCat t lhs rhs both body) (at level 98, right associativity) : term_scope.
+
+(* should probably be sets *)
+Fixpoint fv e : list ident :=
+  match e with
+  | TmSink | TmUnit => nil
+  | TmVar x => cons x nil
+  | TmComma e1 e2 | TmSemic e1 e2 => fv e1 ++ fv e2
+  | TmLet x e e' => fv e ++ remove equiv_dec x (fv e')
+  | TmLetPar x y z e | TmLetCat _ x y z e => cons z (remove equiv_dec x (remove equiv_dec y (fv e)))
+  end.
+
+Inductive wf : term -> Prop :=
+  | wf_TmSink : wf sink
+  | wf_TmUnit : wf unit
+  | wf_TmVar : forall x, wf x
+  | wf_TmComma : forall e e',
+      wf e ->
+      wf e' ->
+      wf (e , e')
+  | wf_TmSemic : forall e e',
+      wf e ->
+      wf e' ->
+      wf (e ; e')
+  | wf_TmLet : forall x e e',
+      wf e ->
+      wf e' ->
+      wf (TmLet x e e')
+  | wf_TmLetPar : forall x y z e,
+      wf e ->
+      x <> y ->
+      y <> z ->
+      x <> z ->
+      wf (TmLetPar x y z e)
+.
 
 (*
 Fixpoint eq_tm lhs rhs :=
