theories/Typing.v
@@ -1,45 +1,49 @@
 From LambdaST Require Import
   Context
   Terms
-  Types.
+  Types
+  Hole.
+From Coq Require Import
+  List.
+
+From Hammer Require Import Tactics.
 
 Declare Scope typing_scope.
 
 Reserved Notation "G '|-' x '\in' T" (at level 98).
 
-(*
 Inductive Typed : context -> term -> type -> Prop :=
   | T_Par_R : forall G e1 e2 s t,
       G |- e1 \in s ->
       G |- e2 \in t ->
       G |- (TmComma e1 e2) \in (TyPar s t)
-  | T_Par_L : forall Gxy Gz x y z s t e r,
-      FindReplace (CtxComma (CtxHasTy x s) (CtxHasTy y t)) (CtxHasTy z (TyPar s t)) Gxy Gz ->
-      Gxy |- e \in r ->
-      Gz |- (TmLetPar x y z e) \in r
+  | T_Par_L : forall G x y z s t e r,
+      fill G (CtxComma (CtxHasTy x s) (CtxHasTy y r)) |- e \in r ->
+      fill G (CtxHasTy z (TyPar s t)) |- (TmLetPar x y z e) \in r
   | T_Cat_R : forall G D e1 e2 s t,
       G |- e1 \in s ->
       D |- e2 \in t ->
       (CtxSemic G D) |- (e1; e2) \in (TyDot s t)
-  | T_Cat_L : forall Gxy Gz x y z s t e r,
-      FindReplace (CtxSemic (CtxHasTy x s) (CtxHasTy y t)) (CtxHasTy z (TyDot s t)) Gxy Gz ->
-      Gxy |- e \in r ->
-      Gz |- (TmLetCat x y z e) \in r
+  | T_Cat_L : forall G x y z s t e r,
+      fill G (CtxSemic (CtxHasTy x s) (CtxHasTy y r)) |- e \in r ->
+      fill G (CtxHasTy z (TyPar s t)) |- (TmLetCat t x y z e) \in r
   | T_Eps_R : forall G,
       G |- sink \in eps
   | T_One_R : forall G,
       G |- unit \in 1
   | T_Var : forall G x s,
-      Contains (CtxHasTy x s) G ->
-      G |- (TmVar x) \in s
+      fill G (CtxHasTy x s) |- (TmVar x) \in s
   | T_SubCtx : forall G G' e s,
-      Contains G' G ->
+      (* Contains G' G -> *)
       G' |- e \in s ->
       G |- e \in s
-  | T_Let : forall Gxs GD D x e e' s t,
-      FindReplace (CtxHasTy x s) D Gxs GD ->
+  | T_Let : forall G D x e e' s t,
       D |- e \in s ->
-      Gxs |- e' \in t ->
-      GD |- TmLet x e e' \in t
+      fill G (CtxHasTy x s) |- e' \in t ->
+      fill G D |- TmLet x e e' \in t
 where "G '|-' x '\in' T" := (Typed G x T).
-*)
+
+Theorem typing_fv : forall G e s,
+    G |- e \in s ->
+    forall x, In x (fv e) -> In x (vars_in G).
+Admitted.
