theories/Context.v
@@ -4,7 +4,8 @@ From Coq Require Import
 From LambdaST Require Import
   Ident
   Terms
-  Types.
+  Types
+  ListUtil.
 
 Inductive context : Set :=
   | CtxEmpty
@@ -19,3 +20,20 @@ Fixpoint vars_in ctx : list ident :=
   | CtxHasTy x _ => cons x nil
   | CtxComma lhs rhs | CtxSemic lhs rhs => vars_in lhs ++ vars_in rhs
   end.
+
+Inductive wf_ctx : context -> Prop :=
+| wf_CtxEmpty : wf_ctx CtxEmpty
+| wf_CtxHasTy : forall x t, wf_ctx (CtxHasTy x t)
+| wf_CtxComma : forall g g',
+    wf_ctx g ->
+    wf_ctx g' ->
+    disjoint (vars_in g) (vars_in g') ->
+    wf_ctx (CtxComma g g')
+| wf_CtxSemic : forall g g',
+    wf_ctx g ->
+    wf_ctx g' ->
+    disjoint (vars_in g) (vars_in g') ->
+    wf_ctx (CtxSemic g g')
+.
+
+(* will need to prove that context derivatives preserve this... *)
