theories/Ident.v
@@ -1,5 +1,7 @@
 From Coq Require Import
-  Strings.String.
+  Strings.String
+  Classes.EquivDec
+  Logic.Decidable.
 
 Definition ident : Set := string.
 
@@ -7,3 +9,8 @@ Bind Scope string_scope with ident.
 
 Definition eq_id : ident -> ident -> bool := eqb.
 Notation "a '=i' b" := (eq_id a b) (at level 98).
+
+Instance EqDec : EqDec Ident.ident eq :=
+{
+  equiv_dec x y := string_dec x y
+}.
