theories/Invert.v
@@ -1,1 +1,2 @@
+(* use sinvert :) *)
 Ltac invert H := inversion H; subst; clear H.
