theories/ListUtil.v
@@ -1,0 +1,14 @@
+From Coq Require Import
+  List
+  String.
+
+From Hammer Require Import Tactics.
+
+Definition disjoint {A : Type} (xs : list A) (ys : list A) : Prop :=
+  forall x, (In x xs -> ~In x ys) /\ (In x ys -> ~ In x xs).
+
+Theorem disjoint_sym {A : Type} : forall (xs : list A) ys, disjoint xs ys -> disjoint ys xs.
+Proof.
+sfirstorder.
+Qed.
+  
