theories/SemSound.v
@@ -1,0 +1,19 @@
+From LambdaST Require Import
+    Terms
+    Semantics
+    Typing
+    Prefix
+    Environment.
+Require Import Coq.Program.Equality.
+
+From Hammer Require Import Tactics.
+
+
+Theorem soundout : forall G e e' s eta p,
+    Typed G e s ->
+    EnvTyped eta G ->
+    Step eta e e' p ->
+    PfxTyped p s
+.
+Proof.
+Admitted.
